src/Lean/Meta/Tactic/Simp/BuiltinSimprocs/BitVec.lean
@@ -165,6 +165,8 @@ builtin_dsimproc [simp, seval] reduceGetLsb (getLsbD _ _) := reduceGetBit ``getL
 builtin_dsimproc [simp, seval] reduceGetMsb (getMsbD _ _) := reduceGetBit ``getMsbD getMsbD
 /-- Simplification procedure for `clz` (count leading zeros) on `BitVec`. -/
 builtin_dsimproc [simp, seval] reduceClz (clz _) := reduceUnary ``BitVec.clz 2 BitVec.clz
+/-- Simplification procedure for `popCount` (population count) on `BitVec`. -/
+builtin_dsimproc [simp, seval] reducePopCnt (popCnt _) := reduceUnary ``BitVec.popCnt 2 BitVec.popCnt
 
 /-- Simplification procedure for `getElem`  on `BitVec`. -/
 builtin_dsimproc [simp, seval] reduceGetElem ((_ : BitVec _)[_]) := fun e => do
